some progress

system_f_sub.lean
@@ -1,5 +1,76 @@
 import data.list.basic
 
+lemma {u} if_pos' {c : Prop} {h : decidable c} (hc : c) {α : Sort u} {t e : α} : (ite c t e) = t :=
+match h with
+| (is_true  hc)  := rfl
+| (is_false hnc) := absurd hc hnc
+end
+
+lemma {u} if_neg' {c : Prop} {h : decidable c} (hnc : ¬c) {α : Sort u} {t e : α} : (ite c t e) = e :=
+match h with
+| (is_true hc)   := absurd hc hnc
+| (is_false hnc) := rfl
+end
+
+@[congr]
+lemma {u} if_simp_congr' {α : Sort u} {b c : Prop} {dec_b : decidable b} {x y u v : α}
+                    (h_c : b ↔ c) (h_t : x = u) (h_e : y = v) :
+        ite b x y = (@ite c (decidable_of_decidable_of_iff dec_b h_c) α u v) :=
+@if_ctx_simp_congr α b c dec_b x y u v h_c (λ h, h_t) (λ h, h_e)
+local attribute [-congr] if_simp_congr
+
+lemma nat.succ_lt_succ_iff (n m : ℕ) : n.succ < m.succ ↔ n < m :=
+⟨nat.lt_of_succ_lt_succ, nat.succ_lt_succ⟩
+
+theorem nat.sub_lt_sub_right : Π {n m k : ℕ} (h₁ : n < m) (h₂ : k ≤ n), n - k < m - k
+| n     m     0     h₁ h₂ := h₁
+| (n+1) (m+1) (k+1) h₁ h₂ := by simp; apply nat.sub_lt_sub_right (nat.lt_of_succ_lt_succ h₁) (nat.le_of_succ_le_succ h₂)
+
+namespace list
+universe u
+variables {α β : Type u}
+@[simp]
+lemma nth_map (xs : list α) (f : α → β) (i : ℕ) : (xs.map f).nth i = f <$> xs.nth i :=
+begin
+  induction xs generalizing i,
+  { refl },
+  { cases i, { refl },
+    apply ih_1 }
+end
+
+@[simp]
+lemma nth_drop (xs : list α) (i k : ℕ) : (xs.drop k).nth i = xs.nth (i + k) :=
+begin
+  induction xs generalizing k i,
+  { cases k; refl },
+  { cases k, { refl },
+    simp [nat.add_succ],
+    apply ih_1 }
+end
+
+lemma nth_take (xs : list α) (i k : ℕ) : (xs.take k).nth i = if i < k then xs.nth i else none :=
+begin
+  induction xs generalizing k i,
+  { simp [list.nth] },
+  { cases k, { refl },
+    cases i, { refl },
+    simp [list.take, ih_1, nat.succ_lt_succ_iff],
+    apply if_congr; refl }
+end
+
+lemma nth_append (xs ys : list α) (i : ℕ) : (xs ++ ys).nth i =
+  if i < length xs then xs.nth i else ys.nth (i - length xs) :=
+begin
+  induction xs generalizing i,
+  case list.nil { refl },
+  case list.cons x xs { cases i with i,
+    { refl },
+    { simp [ih_1, nat.one_add, nat.succ_lt_succ_iff],
+      apply if_congr; refl }
+  }
+end
+end list
+
 namespace system_f_sub
 
 inductive type
@@ -7,27 +78,59 @@ inductive type
 | top
 | «fun» (domain body : type)
 | abs (bound body : type)
+| mu (rec : type)
 
 open type
 
 local infixr ` →ₛ `:50 := type.fun
 local notation `∀0<: ` t `, ` s := abs t s
 
-def type.lift : ℕ → type → type
-| d (var x) := var (x+d)
-| d top := top
-| d (a →ₛ b) := type.lift d a →ₛ type.lift d b
-| d (∀0<:a, b) := ∀0<:type.lift d a, type.lift d b
+@[simp]
+def type.lift (k : ℕ) : type → opt_param ℕ 0 → type
+| (var x)    d := if x ≥ d then var (x+k) else var x
+| top        d := top
+| (a →ₛ b)   d := a.lift d →ₛ b.lift d
+| (∀0<:a, b) d := ∀0<:a.lift d, b.lift (d+1)
+| (mu a)     d := mu (a.lift (d+1))
 
-def env := list type
+@[simp]
+def type.instantiate : type → type → opt_param ℕ 0 → type
+| (var n)     r d := if n < d then var (n-1) else if n = d then r.lift d else var n
+| top         r d := top
+| (a →ₛ b)    r d := a.instantiate r d →ₛ b.instantiate r d
+| (∀0<: a, b) r d := ∀0<:a.instantiate r d, b.instantiate r (d+1)
+| (mu a)      r d := mu (a.instantiate r (d+1))
+
+def type.expand (a : type) : type :=
+a.instantiate (mu a)
+
+def type.free_range : type → ℕ
+| (var d)     := d + 1
+| top         := 0
+| (a →ₛ b)    := max a.free_range b.free_range
+| (∀0<: a, b) := max a.free_range (b.free_range - 1)
+| (mu a)      := a.free_range - 1
+
+@[reducible]
+def type.closed (t : type) := t.free_range = 0
+
+@[reducible] def env := list type
+
+def env.lift : env → ℕ → opt_param ℕ 0 → env
+| [] k d := []
+| (a::e) k d := a.lift k (d + e.length) :: env.lift e k d
 
 inductive sub : env → type → type → Prop
   notation e ` ⊢ `:40 a ` <: `:40 b:40 := sub e a b
 | var_refl (e x) : e ⊢ var x <: var x
-| env {e x a b} : list.nth e x = some a → e ⊢ b <: a.lift x → e ⊢ var x <: b
+| env {e x a b} : list.nth e x = some a → e ⊢ a.lift (x+1) <: b → e ⊢ var x <: b
 | top (e a) : e ⊢ a <: top
 | «fun» {e a a' b b'} : e ⊢ a' <: a → e ⊢ b <: b' → e ⊢ a →ₛ b <: a' →ₛ b'
 | abs {e a a' b b'} : e ⊢ a' <: a → a'::e ⊢ b <: b' → e ⊢ ∀0<:a, b <: ∀0<:a', b'
+--| mu {e a a'} : (∀ b b', e ⊢ b <: b' → e ⊢ type.instantiate a b <: type.instantiate a' b') → e ⊢ mu a <: mu a'
+| mu_refl (e a) : e ⊢ mu a <: mu a
+| expₗ {e a a'} : e ⊢ type.expand a <: a' → e ⊢ mu a <: a'
+| expᵣ {e a a'} : e ⊢ a <: type.expand a' → e ⊢ a <: mu a'
 
 notation e ` ⊢ `:40 a:41 ` <: `:40 b:40 := sub e a b
 notation a ` <: `:40 b:40 := sub [] a b
@@ -37,6 +140,7 @@ lemma sub.refl : Π e a, e ⊢ a <: a
 | e top        := sub.top e top
 | e (a →ₛ b)   := sub.fun (sub.refl e a) (sub.refl e b)
 | e (∀0<:a, b) := sub.abs (sub.refl e a) (sub.refl _ b)
+| e (mu a)     := sub.mu_refl e a
 
 section
 open lean
@@ -44,16 +148,19 @@ open lean.parser
 open interactive
 open interactive.types
 
-open expr (app pi const)
+open expr (app pi const lam)
 
 reserve notation `⟦ₛ`:1000
+def mu_helper := 0
+notation `μ ` binder `, ` a:scoped := mu_helper a
 
 private meta def aux : ℕ → ℕ → pexpr → parser pexpr
 | d d' (expr.var n) := let n := n - d' in pure ``(var %%(reflect n))
-| d d' (expr.const ``top _) := pure ``(top)
+| d d' (const n ls) := pure $ const n ls
+| d d' (app (const ``mu_helper _) (lam _ _ _ a)) := do a ← aux (d+1) d' a, pure ``(mu %%a)
 | d d' (expr.local_const n m bi t) := pure $ ``(type.lift  %%(reflect d) %%(expr.local_const n m bi t))
 -- ``(∀ x <: %%a, %%b)
-| d d' (pi _ _ _ (pi _ _ (app (app (app (const `sub []) _) (expr.var 0)) a) b)) :=
+| d d' (pi _ _ _ (pi _ _ (app (app (app (const `system_f_sub.sub []) _) (expr.var 0)) a) b)) :=
 do a ← aux (d+1) (d'+1) a, b ← aux (d+1) (d'+1) b, pure ``(∀0<:%%a, %%b)
 | d d' (expr.pi _ _ dom b) :=
 if (@unchecked_cast _ expr b).has_var_idx 0 then
@@ -62,9 +169,10 @@ if (@unchecked_cast _ expr b).has_var_idx 0 then
      do dom ← aux d d' dom, b ← aux d (d'+1) b, pure ``(%%dom →ₛ %%b)
 | d d' e := match e.get_structure_instance_info with
   | some info :=
-    let fields := (info.field_names.zip info.field_values).map (λ ⟨n, v⟩,
-      ``(⟨%%(const (`labels ++ n) [] : pexpr), %%v⟩)) in
-    pure ```(record %%(fields.foldr (λ e f, ``(%%e::%%f)) ``([])))
+    do fields ← (info.field_names.zip info.field_values).mmap (λ ⟨n, v⟩,
+      do v ← aux d d' v,
+         pure ``(⟨%%(const (`system_f_sub.labels ++ n) [] : pexpr), %%v⟩)),
+    pure (app (const `system_f_sub.record []) (fields.foldr (λ e f, ``(%%e::%%f)) ``([])))
   | _ := tactic.fail format!"unsupported sub-expression {e.to_raw_fmt}"
   end
 
@@ -87,13 +195,184 @@ example : False <: Bool := by repeat {constructor}
 def prod (a b : type) := ⟦ₛ ∀ r, (a → b → r) → r ⟧
 infix ` ×ₛ `:45 := prod
 
-lemma sub_iff_sub_lift {e k a b} : e ⊢ type.lift k a <: type.lift k b ↔ e.drop k ⊢ a <: b := sorry
+attribute [simp] nat.succ_le_succ
 
-lemma prod.sub {e a a' b b'} :
+lemma lift_lift {k k' d d'} (a : type) : d ≤ d' → d' ≤ k + d → (a.lift k d).lift k' d' = a.lift (k + k') d :=
+begin
+  intros, induction a generalizing d d',
+  all_goals { simp [*,type.lift] },
+  case type.var {
+    by_cases idx ≥ d,
+    { simp [ge, h, type.lift, le_trans ‹d' ≤ k + d› (add_le_add_left h _)] },
+    { have : ¬d' ≤ idx, from λ hcontr, h (le_trans ‹d ≤ d'› hcontr),
+      simp [ge, h, type.lift, this] }
+  },
+  all_goals { simp [nat.add_one, *] }
+end
+
+@[simp]
+lemma lift_lift' (k k') (a : type) : (a.lift k).lift k' = a.lift (k + k') :=
+lift_lift _ dec_trivial dec_trivial
+
+lemma lift_lift2 (k k' d d') (a : type) : k + d ≤ d' → (a.lift k d).lift k' d' = (a.lift k' (d' - k)).lift k d :=
+begin
+  intro h, induction a generalizing d d',
+  all_goals {
+    have : k ≤ d', from le_trans (nat.le_add_right _ _) ‹k + d ≤ d'›,
+    simp [*,type.lift] },
+  case type.var {
+    by_cases idx ≥ d,
+    { by_cases d' ≤ k + idx with h',
+      { have : d' - k ≤ k + idx - k, from nat.sub_le_sub_right h' k,
+        simp [nat.add_sub_cancel_left] at this,
+        simp [ge, h, type.lift, h', this, le_add_of_nonneg_of_le (nat.zero_le _) h] },
+      { have : ¬ d' - k ≤ idx, begin
+          assume hcontr, apply h',
+          have : d' - k + k ≤ idx + k, from nat.add_le_add_right hcontr k,
+          simp [nat.sub_add_cancel ‹k ≤ d'›] at this,
+          simp [this],
+        end,
+        simp [ge, h, type.lift, h', this] }
+    },
+    { simp [ge, h],
+      have : ¬d' - k ≤ idx, begin
+        have : k + idx < k + d, from add_lt_add_left (lt_of_not_ge h) _,
+        have : idx + k < k + d, by simp [this],
+        have : d' > idx + k, from lt_of_lt_of_le this ‹k + d ≤ d'›,
+        have : d' - k > idx + k - k, from nat.sub_lt_sub_right this (nat.le_add_left _ _),
+        simp only [nat.add_sub_cancel] at this,
+        exact not_le_of_gt this,
+      end,
+      have : d ≤ d', from le_trans (nat.le_add_left _ _) ‹k + d ≤ d'›,
+      have : ¬d' ≤ idx, from not_le_of_gt (lt_of_lt_of_le (lt_of_not_ge h) this),
+      simp [*, if_neg' h, type.lift, if_neg' this] }
+  },
+  case type.abs {
+    rw [ih_2, add_comm, nat.add_sub_assoc ‹k ≤ d'›],
+    { simp [nat.add_one, *] } },
+  case type.mu {
+    rw [ih_1, add_comm, nat.add_sub_assoc ‹k ≤ d'›],
+    { simp [nat.add_one, *] } }
+end
+
+lemma nat.succ_le_iff_lt (n m : ℕ) : n.succ ≤ m ↔ n < m := ⟨nat.succ_le_of_lt, nat.lt_of_succ_le⟩
+
+@[simp]
+lemma instantiate_lift (a b : type) (k d d') : d' < d → (a.lift k (d + 1)).instantiate (b.lift k d) d' = (a.instantiate b d').lift k d :=
+begin
+  intro, induction a generalizing d d',
+  all_goals { simp },
+  case type.var {
+    simp [nat.add_one, ge, nat.succ_le_iff_lt],
+    by_cases d < idx,
+    { have : ¬ k + idx < d', from sorry,
+      have : k + idx ≠ d', from sorry,
+      have : d' < idx, from lt_trans ‹d' < d› ‹d < idx›,
+      simp [*, ge, le_of_lt h, not_lt_of_gt this, (ne_of_lt this).symm] },
+    { simp [h],
+      by_cases idx < d' with h',
+      { have : ¬ idx - 1 ≥ d, from sorry,
+        simp * },
+      { by_cases idx = d',
+        { simp [*] } }
+    }
+  }
+end
+
+@[simp]
+lemma expand_lift (k d) (a : type) : (a.lift k (d+1)).expand = a.expand.lift k d :=
+by simp [type.expand]; rw [←type.lift, instantiate_lift]
+
+@[simp]
+lemma env.length_lift (e : env) (k d) : (e.lift k d).length = e.length :=
+by induction e; simp [env.lift, *]
+
+@[simp]
+lemma option_has_map_map_none {α β : Type} (f : α → β) : f <$> none = none := rfl
+
+@[simp]
+lemma option_has_map_map_some {α β : Type} (f : α → β) (x : α) : f <$> some x = f x := rfl
+
+@[simp]
+lemma env.nth_lift {e : env} (k d i) : (e.lift k d).nth i = (λ a : type, a.lift k (d + (e.length - 1 - i))) <$> e.nth i :=
+begin
+  induction e generalizing i,
+  { simp [env.lift] },
+  { simp [list.nth],
+    cases i with i,
+    { simp [env.lift, list.nth, nat.add_sub_cancel_left], refl },
+    { simp [env.lift, ih_1, nat.add_sub_cancel_left, nat.sub_sub] }
+  }
+end
+
+/-@[simp]
+lemma lift_zero (a : type) : a.lift 0 = a :=
+by induction a; simp [*, type.lift]-/
+
+lemma sub_insert {e₁ e₂ : env} {a b c} : e₁ ++ e₂ ⊢ a <: b → e₁.lift 1 ++ c::e₂ ⊢ a.lift 1 e₁.length <: b.lift 1 e₁.length :=
+begin
+  generalize he' : e₁ ++ e₂ = e',
+  intro h, induction h generalizing c e₁,
+  all_goals { simp [type.lift, -add_comm], try {constructor; done} },
+  case sub.var_refl {
+    by_cases x ≥ e₁.length,
+    { simp [if_pos h], apply sub.var_refl },
+    { simp [if_neg h], apply sub.var_refl }
+  },
+  case sub.env e' x a b h₁ h₂ ih {
+    subst e',
+    by_cases x ≥ e₁.length,
+    { simp [if_pos h], apply sub.env,
+      { have : ¬ (x + 1 < e₁.length), from
+          λ hcontr, not_lt_of_ge h (nat.lt_of_succ_lt hcontr),
+        simp [list.nth_append, if_neg' this, nat.sub_add_comm h, -add_comm, list.nth],
+        simp [list.nth_append, if_neg (not_lt_of_ge h)] at h₁,
+        apply h₁ },
+      { have ih := ih rfl,
+        rw lift_lift _ (nat.zero_le _) (nat.le_succ_of_le h) at ih,
+        apply ih }
+    },
+    { simp [if_neg h], apply sub.env,
+      { simp [list.nth_append, if_pos' (lt_of_not_ge h)] at ⊢ h₁,
+        -- HACK
+        show _ = some (a.lift 1 (e₁.length - 1 - x)),
+        simp [h₁], refl },
+      { have ih := ih rfl,
+        rw lift_lift2 at ih,
+        { rw [nat.sub_sub, nat.one_add], apply ih },
+        { apply nat.succ_le_of_lt (lt_of_not_ge h) }
+      }
+    }
+  },
+  case sub.abs {
+    have ih_2 := @ih_2 c (a'::e₁),
+    apply sub.abs; simp [*, env.lift] at *
+  },
+  case sub.fun {
+    apply sub.fun (ih_1 he') (ih_2 he')
+  },
+  case sub.expₗ {
+    apply sub.expₗ,
+    simp only [expand_lift],
+    apply ih_1 he'
+  },
+  case sub.expᵣ {
+    apply sub.expᵣ,
+    simp only [expand_lift],
+    apply ih_1 he'
+  }
+end
+
+lemma prod.sub {e : env} {a a' b b'} :
   e ⊢ a <: a' →
   e ⊢ b <: b' →
   e ⊢ a ×ₛ b <: a' ×ₛ b' :=
-by intros; repeat { any_goals {constructor <|> apply sub_iff_sub_lift.mpr <|> assumption} }
+begin
+  intros,
+  repeat {any_goals {constructor}},
+  apply @sub_insert []; assumption,
+  apply @sub_insert []; assumption
+end
 
 def tuple : list type → type
 | []      := top
@@ -102,7 +381,7 @@ def tuple : list type → type
 lemma {u} list.elem_zip_cons_of_elem_zip {α β : Type u} {a : α} {b : β} {p as bs} : p ∈ list.zip as bs → p ∈ list.zip (a::as) (b::bs) :=
 or.inr
 
-lemma list.sub {e as as'} : list.length as = list.length as' → (∀ p ∈ as.zip as', e ⊢ prod.fst p <: p.2) → e ⊢ tuple as <: tuple as' :=
+lemma list.sub {e : env} {as as'} : list.length as = list.length as' → (∀ p ∈ as.zip as', e ⊢ prod.fst p <: p.2) → e ⊢ tuple as <: tuple as' :=
 begin
   intros hlen helem, induction as generalizing as',
   { cases as', {constructor}, {contradiction} },
@@ -167,15 +446,134 @@ def foo := record [⟨a, int⟩, ⟨b, top⟩]
 def bar := record [⟨a, int⟩, ⟨b, int⟩, ⟨c, int⟩]
 
 open tactic
+--set_option trace.type_context.is_def_eq true
+--set_option trace.simplify true
 example : bar <: foo :=
 record.sub dec_trivial (λ ⟨a, b⟩ h, begin
-  conv at h { reduce, simp },
+  conv at h {
+    find (list.zip _ _) {whnf,reflexivity},
+    simp,
+    find (option.get_or_else _ _) {whnf},
+    find (option.get_or_else _ _) {whnf},
+    find (option.get_or_else _ _) {whnf},
+    find (option.get_or_else _ _) {whnf},
+  },
   cases h with h h; simp [h],
-  { apply sub.top },
   { apply sub.refl },
+  { apply sub.top },
 end)
 
 end
+
+@[simp]
+lemma lift_tuple (as k) : (tuple as).lift k = tuple (as.map (λ a, a.lift k 1)) :=
+begin
+  induction as,
+  { refl },
+  { simp [tuple, prod] }
+end
+
+@[simp]
+lemma instantiate_tuple (as b) : (tuple as).instantiate b = tuple (as.map (λ a, a.instantiate b)) :=
+begin
+  induction as,
+  { refl },
+  { simp [tuple, prod, type.instantiate, ih_1] }
+end
+
+lemma instantiate_record (b fs) : (record fs).instantiate b = record (fs.map (λ ⟨i, a⟩, ⟨i, a.instantiate b⟩)) :=
+begin
+  simp [record, record_list],
+  apply congr_arg,
+  apply congr_fun,
+  { apply congr_arg,
+    apply congr,
+    { apply congr_arg,
+      apply funext, intro i,
+      induction fs,
+      { refl },
+      { simp [list.find], cases a,
+        simp,
+        by_cases idx = i,
+        { simp [function.comp, h, option.get_or_else, has_map.map, option_map, option_bind] },
+        { simp [function.comp, h], apply ih_1 },
+      }
+    },
+    { apply congr_arg,
+      apply congr_arg,
+      apply congr_fun, simp,
+      apply congr_fun,
+      apply congr_arg,
+      apply funext, intro a, cases a with idx ty,
+      simp }
+  }
+end
+
+lemma lift_free_range {t : type} (k m) : t.free_range ≤ m → t.lift k m = t :=
+begin
+  induction t generalizing m,
+  all_goals { simp [type.free_range, type.lift] },
+  { intro h,  simp [if_neg' (not_le_of_gt (nat.lt_of_succ_le h))] },
+  { intro h,
+    have := ih_1 m (le_trans (le_max_left _ _) h),
+    rw [this],
+    have := ih_2 m (le_trans (le_max_right _ _) h),
+    rw [this] },
+  { intro h,
+    have := ih_1 m (le_trans (le_max_left _ _) h),
+    rw [this],
+    have : body.lift k (m+1) = body, {
+      apply ih_2 (m+1),
+      have : body.free_range - 1 ≤ m, from le_trans (le_max_right _ _) h,
+      show body.free_range ≤ m + 1, from nat.le_succ_of_pred_le this,
+    },
+    rw [this] },
+  { intro h,
+    have := ih_1 (m+1) (nat.le_succ_of_pred_le h),
+    rw [this] }
+end
+
+lemma lift_closed {t : type} (k) : t.closed → (t.lift k) = t :=
+begin
+  intro h, apply lift_free_range,
+  simp [type.closed] at h, simp [h]
+end
+
+lemma left_le_of_max_le {a b c : ℕ} : max a b ≤ c → a ≤ c :=
+begin
+  intro h,
+  by_cases a ≤ b with ab,
+  { simp [max, ab] at h, apply le_trans ab h },
+  { simp [max, ab] at h, apply h }
+end
+
+lemma right_le_of_max_le {a b c : ℕ} : max a b ≤ c → b ≤ c :=
+begin
+  intro h,
+  by_cases a ≤ b with ab,
+  { simp [max, ab] at h, apply h },
+  { simp [max, ab] at h, apply le_trans (le_of_not_le ab) h }
+end
+
+lemma instantiate_free_range {t t' : type} {d} : t.free_range ≤ d → t.instantiate t' d = t :=
+begin
+  induction t generalizing d,
+  all_goals { simp [type.instantiate, type.free_range] },
+  { intro h, simp [if_neg (ne_of_lt (nat.lt_of_succ_le h))] },
+  { intro h, rw[ih_1 (le_trans (left_le_of_max_le h) (le_refl _)),
+                ih_2 (le_trans (right_le_of_max_le h) (le_refl _))] },
+  { intro h, rw[ih_1 (le_trans (left_le_of_max_le h) (le_refl _)),
+                ih_2 (le_trans (nat.le_succ_of_pred_le (right_le_of_max_le h)) (le_refl _))] },
+  { intro h, rw[ih_1 (le_trans (nat.le_succ_of_pred_le h) (le_refl _))] },
+end
+
+@[simp]
+lemma instantiate_closed {t t' : type} : t.closed → t.instantiate t' = t :=
+begin
+  intro h, apply instantiate_free_range,
+  simp [type.closed] at h, simp [h]
+end
+
 end system_f_sub
 
 section
@@ -208,117 +606,23 @@ do base ← ident,
    let is := is ++ idecl.intros.map (λ e, (e.local_uniq_name, e.local_type)),
    set_env $ env.add_namespace new,
    add_inductive new ls p ty is
-end
 
-namespace system_f_sub_mu
---extend_inductive type with type
---| μ : type → type
+meta def dunfold_productive (cfg : delta_config := {}) : conv unit :=
+let unfold (u : unit) (e : expr) : tactic (unit × expr × bool) := do
+  (expr.const f_name _) ← return e.get_app_fn,
+  es ← get_eqn_lemmas_for ff f_name,
+  guard $ es.length > 1,
+  sl ← es.mfoldl simp_lemmas.add_simp simp_lemmas.mk,
+  new_e ← sl.drewrite e,
+  return (u, new_e, tt)
+in do e ← target,
+      (c, new_e) ← dsimplify_core () (λ c e, failed) unfold e {max_steps := cfg.max_steps, canonize_instances := cfg.visit_instances},
+      change new_e
 
-inductive type
-| var (idx : ℕ)
-| top
-| «fun» (domain body : type)
-| abs (bound body : type)
-| mu (rec : type)
+meta def delta_target (cs : list name) (cfg : delta_config := {}) : tactic unit :=
+do t ← target, delta cs t cfg >>= unsafe_change
 
-open type
-
-local infixr ` →ₛ `:50 := type.fun
-local notation `∀0<: ` t `, ` s := abs t s
-
-def type.instantiate_aux (b : type) : ℕ → type → type
-| d (var n) := if n = d then b else var n
-| d top     := top
-| d (a →ₛ b) := type.instantiate_aux d a →ₛ type.instantiate_aux d b
-| d (∀0<: a, b) := ∀0<:type.instantiate_aux d a, type.instantiate_aux (d+1) b
-| d (mu a) := mu (type.instantiate_aux (d+1) a)
-
-def type.instantiate (a b : type) := type.instantiate_aux b 0 a
-
-def type.expand (a : type) : type :=
-a.instantiate (mu a)
-
-inductive relμ : type → type → Prop
-  infix ` ~ `:40 := relμ
-| expand {a b : type} : a.expand ~ b → mu a ~ b
-| retract {a b : type} : a ~ b.expand → a ~ mu b
-| var (n) : var n ~ var n
-| top : top ~ top
-| «fun» {d d' b b'} : d ~ d' → b ~ b' → d →ₛ b ~ d' →ₛ b'
-| abs {a a' b b'} : a ~ a' → b ~ b' → abs a b ~ abs a' b'
-| mu {a a'} : a ~ a' → mu a ~ mu a'
-
-local infix ` ~ `:40 := relμ
-
-lemma relμ.refl (a) : a ~ a := sorry
-
-def type' := quot relμ
-instance : setoid type := ⟨relμ, sorry⟩
-
-example : ⟦ mu (top →ₛ var 0) ⟧ = ⟦ top →ₛ mu (top →ₛ var 0) ⟧ :=
-begin
-  apply quotient.sound,
-  apply relμ.expand,
-  apply relμ.refl
-end
-
-def prod (a b : type) := ∀0<:top, (a.lift 1 →ₛ b.lift 1 →ₛ var 0) →ₛ var 0 --⟦ₛ ∀ r, (a → b → r) → r ⟧
-infix ` ×ₛ `:45 := prod
-
-def tuple : list type → type
-| []      := top
-| (a::as) := a ×ₛ tuple as
-
-section records
-structure field :=
-(idx : ℕ)
-(type : type)
-
-def record_list (fields : list field) : list type :=
-let max_idx := (fields.map field.idx).foldr max 0 in
-(list.range (max_idx+1)).map (λ i, (field.type <$> fields.find (λ f, f.idx = i)).get_or_else top)
-
-def record (fields : list field) : type :=
-tuple (record_list fields ++ [top])
-end records
-
-section
-open lean
-open lean.parser
-open interactive
-open interactive.types
-
-open expr (app pi const lam)
-
-reserve notation `⟦ₛ`:1000
-def mu_helper := 0
-notation `μ ` binder `, ` a:scoped := mu_helper a
-
-private meta def aux : ℕ → ℕ → pexpr → parser pexpr
-| d d' (expr.var n) := let n := n - d' in pure ``(var %%(reflect n))
-| d d' (expr.const n ls) := pure $ const n ls
-| d d' (app (const ``mu_helper _) (lam _ _ _ a)) := do a ← aux (d+1) d' a, pure ``(mu %%a)
-| d d' (expr.local_const n m bi t) := pure $ ``(type.lift  %%(reflect d) %%(expr.local_const n m bi t))
--- ``(∀ x <: %%a, %%b)
-| d d' (pi _ _ _ (pi _ _ (app (app (app (const `sub []) _) (expr.var 0)) a) b)) :=
-do a ← aux (d+1) (d'+1) a, b ← aux (d+1) (d'+1) b, pure ``(∀0<:%%a, %%b)
-| d d' (expr.pi _ _ dom b) :=
-if (@unchecked_cast _ expr b).has_var_idx 0 then
-     do b ← aux (d+1) d' b, pure ``(∀0<:top, %%b)
-   else
-     do dom ← aux d d' dom, b ← aux d (d'+1) b, pure ``(%%dom →ₛ %%b)
-| d d' e := match e.get_structure_instance_info with
-  | some info :=
-    do fields ← (info.field_names.zip info.field_values).mmap (λ ⟨n, v⟩,
-      do v ← aux d d' v,
-         pure ``(⟨%%(const (`system_f_sub_mu.labels ++ n) [] : pexpr), %%v⟩)),
-    pure ``(record %%(fields.foldr (λ e f, ``(%%e::%%f)) ``([])))
-  | _ := tactic.fail format!"unsupported sub-expression {e.to_raw_fmt}"
-  end
-
-@[user_notation]
-meta def interpret_notation (_ : parse $ tk "⟦ₛ") (e : parse $ parser.pexpr 0 <* tk "⟧") : parser pexpr :=
-do e ← aux 0 0 e, pure ``(⟦%%e⟧)
+run_cmd add_interactive [`dunfold_productive] `conv.interactive
 end
 
 example : ⟦ₛ μ a, top → a ⟧ = ⟦ₛ top → μ a, top → a ⟧ :=
